src/StateRA.v
@@ -2,7 +2,7 @@ From sflib Require Import sflib.
 From Paco Require Import paco.
 From Fairness Require Import PCM ITreeLib pind.
 Require Import Program.
-From Fairness Require Import IProp IPM Weakest.
+From Fairness Require Import IProp IPM.
 From Fairness Require Import PCM MonotonePCM ThreadsRA ModSim FairBeh.
 
 Set Implicit Arguments.
@@ -19,6 +19,7 @@ Section INVARIANT.
   Definition stateTgtRA: URA.t := Auth.t (Excl.t state_tgt).
   Definition identSrcRA: URA.t := Auth.t (Excl.t (imap ident_src wf_src)).
   Definition identTgtRA: URA.t := Auth.t (Excl.t (imap ident_tgt nat_wf)).
+  Definition identThsRA: URA.t := Auth.t (Excl.t (imap thread_id nat_wf)).
 
   Context `{MONORA: @GRA.inG monoRA Σ}.
   Context `{THSRA: @GRA.inG ths_RA Σ}.
@@ -26,6 +27,7 @@ Section INVARIANT.
   Context `{STATETGT: @GRA.inG stateTgtRA Σ}.
   Context `{IDENTSRC: @GRA.inG identSrcRA Σ}.
   Context `{IDENTTGT: @GRA.inG identTgtRA Σ}.
+  Context `{IDENTTHS: @GRA.inG identThsRA Σ}.
 
   Definition default_I: TIdSet.t -> (@imap ident_src wf_src) -> (@imap (sum_tid ident_tgt) nat_wf) -> state_src -> state_tgt -> iProp :=
     fun ths im_src im_tgt st_src st_tgt =>
@@ -38,5 +40,7 @@ Section INVARIANT.
         (OwnM (Auth.black (Excl.just im_src: @Excl.t (imap ident_src wf_src)): identSrcRA))
         **
         (OwnM (Auth.black (Excl.just (imap_proj_id2 im_tgt): @Excl.t (imap ident_tgt nat_wf)): identTgtRA))
+        **
+        (OwnM (Auth.black (Excl.just (imap_proj_id1 im_tgt): @Excl.t (imap thread_id nat_wf)): identThsRA))
   .
 End INVARIANT.
